Capless/Subst/Capture/Typing.lean
@@ -14,4 +14,22 @@ theorem Typed.copen
   apply? Typed.csubst
   apply? CVarSubst.open
 
+theorem Typed.cinstantiate {Γ : Context n m k}
+  (h : Typed (Γ.cvar CBinding.bound) t E) :
+  Typed (Γ.cvar (CBinding.inst C)) t E := by
+  rw [<- Term.crename_id (t := t), <- EType.crename_id (E := E)]
+  apply? Typed.csubst
+  apply? CVarSubst.instantiate
+
+theorem Typed.cinstantiate_extvar {Γ : Context n m k}
+  (h : Typed ((Γ.cvar CBinding.bound).var P) t E) :
+  Typed ((Γ.cvar (CBinding.inst C)).var P) t E := by
+  rw [<- Term.crename_id (t := t), <- EType.crename_id (E := E)]
+  apply? Typed.csubst
+  conv =>
+    arg 3
+    rw [<- CType.crename_id (T := P)]
+  apply CVarSubst.ext
+  apply CVarSubst.instantiate
+
 end Capless
